Refactor eliminate_algebraic to make functional
Separate axioms into separate functions
Make functional - reduce amount of state (can prob eliminate entirely)
Much easier to reason about - can refer to axioms directly
Replace folds with maps when possible

proofs/transform/eliminate_algebraic.v
@@ -20,7 +20,7 @@ Record state := mk_state {
   mt_map : amap typesym funsym;       (* from type symbols to selector functions *)
   cc_map : amap funsym funsym;       (* from old constructors to new constructors *)
   cp_map : amap funsym (list funsym);  (* from old constructors to new projections *)
-  pp_map : amap funsym funsym;       (* from old projections to new projections *)
+  (*pp_map : amap funsym funsym;       (* from old projections to new projections *)*)
   (*kept_m : amap typesym (list vty); *)        (* should we keep constructors/projections/Tcase for this type? *)
   (* tp_map : Mid.t (decl*theory_c); skipped tuple symbols *)
   (* inf_ts : Sts.t;               infinite types *)
@@ -35,7 +35,7 @@ Record state := mk_state {
 
 (*Here, we can use coq-record-update*)
 
-#[export] Instance etaX : Settable _ := settable! mk_state <mt_map; cc_map; cp_map; pp_map; no_ind; no_inv; no_sel>.
+#[export] Instance etaX : Settable _ := settable! mk_state <mt_map; cc_map; cp_map; (*pp_map;*) no_ind; no_inv; no_sel>.
 Import RecordSetNotations. 
 
 (*Infer args for functions - hard to get it right*)
@@ -275,11 +275,15 @@ Definition add_param_decl (t: task) (f: funsym) : task :=
 Definition add_axiom (t: task) (n: string) (f: formula) : task :=
   (task_gamma t, (n, f) :: task_delta t, task_goal t).
 
-(*NOTE: will prob need to separate out for proof purposes (e.g. map2 vs fold_left2 and separate function)*)
-Definition add_selector_aux (st: state * task) (ts: typesym) (ty: vty) (csl: list funsym) :=
-  let s := fst st in
-  let tsk := snd st in
-  if s.(no_sel) then (s, tsk) else
+(*In all of these, we separate out the definition of the axioms/funsyms and the
+  "stateful" (in the monadic sense) function that updates the task and state*)
+
+(*The selector axiom for a given typesym and constructor list*)
+(*NOTE: the cc_map is probably the identity map but we still keep it because
+  it is not (for some reason) in the full version*)
+(*TODO: need condition that all funsyms in csl appear in cc_map*)
+Definition selector_axiom (cc_map : amap funsym funsym) 
+  (ts: typesym) (ty: vty) (csl: list funsym) : funsym * list (string * formula) (*list (funsym * formula)?*) :=
   (* declare the selector function *)
   let mt_id : string := ("match_" ++ ts_name ts)%string in
   (*TODO: does it need to be fresh?*)
@@ -287,8 +291,7 @@ Definition add_selector_aux (st: state * task) (ts: typesym) (ty: vty) (csl: lis
   (* let mt_ty = ty_var (create_tvsymbol (id_fresh "a")) in *)
   let mt_al := ty :: rev_map (fun _ => mt_ty) csl in
   let mt_ls := funsym_noconstr_noty mt_id mt_al mt_ty in
-  let mt_map2 := amap_set typesym_eq_dec s.(mt_map) ts mt_ls in
-  let task  := add_param_decl tsk mt_ls in
+  (* let mt_map2 := amap_set typesym_eq_dec s.(mt_map) ts mt_ls in *)
   (* define the selector function *)
   (*Generate new vars*)
   let varnames := gen_names (length csl) "z"%string nil in
@@ -296,7 +299,7 @@ Definition add_selector_aux (st: state * task) (ts: typesym) (ty: vty) (csl: lis
   (* let mt_vs _ = create_vsymbol (id_fresh "z") mt_ty in *)
   (* let mt_vl = List.rev_map mt_vs csl in *)
   let mt_tl := rev_map Tvar mt_vl in
-  let mt_add tsk (cs: funsym) t :=
+  let mt_add (cs: funsym) t :=
     let id := (mt_id ++ "_" ++ (s_name cs))%string in
     (* let id = mt_ls.ls_name.id_string ^ "_" ^ cs.ls_name.id_string in *) 
     (* let pr = create_prsymbol (id_derive id cs.ls_name) in *)
@@ -304,16 +307,37 @@ Definition add_selector_aux (st: state * task) (ts: typesym) (ty: vty) (csl: lis
     let varnames2 := gen_names (length (s_args cs)) "u"%string varnames in
     let vl := rev (combine varnames2 (s_args cs)) in
     (* let vl = List.rev_map (create_vsymbol (id_fresh "u")) cs.ls_args in *)
-    let newcs := amap_get_def funsym_eq_dec (s.(cc_map)) cs id_fs in (*TODO: show have*)
+    let newcs := amap_get_def funsym_eq_dec cc_map cs id_fs in (*TODO: show have*)
     let hd := tfun_infer' newcs (rev_map snd vl) (rev_map Tvar vl) in (*TODO: is return type right? - they say f_ret cs*)
     let hd := tfun_infer' mt_ls ((f_ret cs) :: map snd mt_vl) (hd :: mt_tl) in
     let vl := rev_append mt_vl (rev vl) in
     let ax := fforalls vl (Feq mt_ty hd t) in
-    add_axiom tsk id ax
+    (id, ax)
   in 
-  let task := fold_left2 mt_add csl mt_tl tsk in
+  (mt_ls, map2 mt_add csl mt_tl).
+
+(*INVARINT: mt_map is fst (selector_axiom)*)
+
+Definition add_task_axioms (t: task) (axs: list (string * formula)) : task :=
+  fold_left (fun acc x => add_axiom acc (fst x) (snd x)) axs t.
+
+(*NOTE: will prob need to separate out for proof purposes (e.g. map2 vs fold_left2 and separate function)*)
+Definition add_selector_aux (st: state * task) (ts: typesym) (ty: vty) (csl: list funsym) :=
+  let s := fst st in
+  let tsk := snd st in
+  if s.(no_sel) then (s, tsk) else
+  let sel := selector_axiom s.(cc_map) ts ty csl in
+  let mt_ls := fst sel in
+  let axms := snd sel in
+  let tsk := add_param_decl tsk mt_ls in
+  let tsk := add_task_axioms tsk axms in
+  (*update state*)
+  let mt_map2 := amap_set typesym_eq_dec s.(mt_map) ts mt_ls in
   (s <|mt_map := mt_map2|>, tsk).
 
+(*Don't need selector for types with single constructor because trivial.
+  NOTE: does this cause any problems with eliminating singleton types (e.g. user defined tuple)
+  need to see in rewriteT*)
 Definition add_selector (acc : state * task) (ts: typesym) (ty: vty) (x: list funsym) :
   state * task :=
   match x with
@@ -321,47 +345,68 @@ Definition add_selector (acc : state * task) (ts: typesym) (ty: vty) (x: list fu
   | csl => add_selector_aux acc ts ty csl
   end.
 
-Definition add_indexer_aux (st: state * task) (ts: typesym) (ty : vty) (csl : list funsym) : state * task :=
-  let s := fst st in
-  let tsk := snd st in
+Definition mapi {A B: Type} (f: nat -> A -> B) (l: list A) : list B :=
+  map (fun x => f (fst x) (snd x)) (combine (seq 0 (length l)) l).
+
+(*Again, define indexer axiom*)
+Definition indexer_axiom (cc_map : amap funsym funsym)  
+  (ts: typesym) (ty : vty) (csl : list funsym) : funsym * list (string * formula) :=
   (* declare the indexer function *)
   let mt_id := ("index_" ++ (ts_name ts))%string in
   let mt_ls := funsym_noconstr_noty mt_id [ty] vty_int in
-  let tsk  := add_param_decl tsk mt_ls in
   (* define the indexer function *)
-  let mt_add tsk (cs: funsym) idx :=
+  let mt_add idx (cs: funsym) :=
     let id := (mt_id ++ "_" ++ (s_name cs))%string in
     (* let pr = create_prsymbol (id_derive id cs.ls_name) in *)
     let varnames := gen_names (length (s_args cs)) "u" nil in
     let vl := rev (combine varnames (s_args cs)) in
-    let newcs := amap_get_def funsym_eq_dec s.(cc_map) cs id_fs in
+    let newcs := amap_get_def funsym_eq_dec cc_map cs id_fs in
     (*NOTE: THESE TYPES MAY BE WRONG!*)
     let hd := tfun_infer' newcs (rev (map snd vl)) (rev_map Tvar vl) in
     (* let hd = fs_app newcs (List.rev_map t_var vl) (Option.get cs.ls_value) in *)
     let ax := Feq vty_int (tfun_infer' mt_ls (*TODO: what is hd type?*) [(f_ret newcs)] [hd] )  
       (Tconst (ConstInt (Z.of_nat idx))) in
     let ax := fforalls (rev vl) ax in
-    add_axiom tsk id ax
-  in
-  let task := fold_left2' mt_add csl (seq 0 (length csl)) tsk in
-  (s, task).
+    (id, ax) in
+  (mt_ls, mapi mt_add csl). 
+
+Definition add_indexer_aux (st: state * task) (ts: typesym) (ty : vty) (csl : list funsym) : state * task :=
+  let s := fst st in
+  let tsk := snd st in
+  let indexer := indexer_axiom s.(cc_map) ts ty csl in
+  let mt_ls := fst indexer in
+  let axms := snd indexer in
+  (*update task*)
+  let tsk := add_param_decl tsk mt_ls in
+  let tsk := add_task_axioms tsk axms in
+  (s, tsk).
 
 Definition t_neq (ty: vty) (t1 t2: term) : formula :=
   Fnot (Feq ty t1 t2).
 
-Definition add_discriminator (st: state * task) (ts: typesym) (ty: vty) (csl: list funsym) : state * task :=
-  let s := fst st in
-  let tsk := snd st in
-  let d_add (c1: funsym) tsk (c2: funsym) :=
-    let id : string := ((s_name c1) ++ "_" ++ (s_name c2))%string in
+(*Discriminator axioms - there should be O(n^2) - 1 per pair of constructors*)
+
+(*Generic: apply function of type A -> A -> B to each pair (a_i, a_j) of elements in l,
+  where i < j*)
+Fixpoint map_pairs {A B: Type} (f: A -> A -> B) (l: list A) : list B :=
+  match l with
+  | x :: xs => map (f x) xs ++ map_pairs f xs
+  | nil => nil
+  end.
+
+(*Here, only axioms - TODO: do we want to index by funsyms: ie, return (funsym * funsym * formula)*)
+Definition discriminator_axioms (cc_map : amap funsym funsym) (ts: typesym) (ty: vty) (csl: list funsym) : 
+  list (string * formula) :=
+  let d_add (c1: funsym) (c2: funsym) : (string * formula) :=
+    let i : string := ((s_name c1) ++ "_" ++ (s_name c2))%string in
     (* let pr = create_prsymbol (id_derive id ts.ts_name) in *)
     (*Create vars - TODO: does it have to be fresh against some vars?*)
     let ul := rev (combine (gen_names (length (s_args c1)) "u" nil) (s_args c1)) in
     let vl := rev (combine (gen_names (length (s_args c2)) "v" nil) (s_args c2)) in
     (* let ul := rev_map (create_vsymbol (id_fresh "u")) c1.ls_args in
     let vl = List.rev_map (create_vsymbol (id_fresh "v")) c2.ls_args in *)
-    let newc1 := amap_get_def funsym_eq_dec (s.(cc_map)) c1 id_fs in
-    let newc2 := amap_get_def funsym_eq_dec (s.(cc_map)) c2 id_fs in
+    let newc1 := amap_get_def funsym_eq_dec (cc_map) c1 id_fs in
+    let newc2 := amap_get_def funsym_eq_dec (cc_map) c2 id_fs in
     let t1 := tfun_infer' newc1 (rev (map snd ul)) (rev_map Tvar ul) in
     let t2 := tfun_infer' newc2 (rev (map snd vl)) (rev_map Tvar vl) in
     (* let t1 = fs_app newc1 (List.rev_map t_var ul) ty in
@@ -369,19 +414,18 @@ Definition add_discriminator (st: state * task) (ts: typesym) (ty: vty) (csl: li
     let ax := t_neq ty t1 t2 in
     let ax := fforalls (rev vl) ax in
     let ax := fforalls (rev ul) ax in
-    add_axiom tsk id ax 
-    (* let ax = t_forall_close (List.rev vl) [[t2]] ax in
-    let ax = t_forall_close (List.rev ul) [[t1]] ax in
-    add_prop_decl task Paxiom pr ax *)
+    (i, ax)
   in
-  let fix dl_add task l := 
-    match l with
-    | c :: cl => dl_add (fold_left (d_add c) cl task) cl
-    | _ => task
-    end
-  in
-  (s, dl_add tsk csl).
+  map_pairs d_add csl.
 
+
+Definition add_discriminator (st: state * task) (ts: typesym) (ty: vty) (csl: list funsym) : state * task :=
+  let s := fst st in
+  let tsk := snd st in
+  let axs := discriminator_axioms s.(cc_map) ts ty csl in
+  (s, add_task_axioms tsk axs).
+
+(*TODO: see if we want to do this still - are there types with more than 16 constructors?*)
 Definition add_indexer (acc: state * task) (ts: typesym) (ty: vty) (cs: list funsym) := 
   match cs with
   | [_] => acc
@@ -390,102 +434,115 @@ Definition add_indexer (acc: state * task) (ts: typesym) (ty: vty) (cs: list fun
     else acc
   end.
 
-Definition mapi {A B: Type} (f: nat -> A -> B) (l: list A) : list B :=
-  map (fun x => f (fst x) (snd x)) (combine (seq 0 (length l)) l).
-
 (*NOTE: complete_projections just copies over projections if they exist.
   We do not have any projections in our data, so we only implement the "None" case.
   TODO: we will need a predicate/typing rule asserting that projection is correct if it exists
   or something (not sure exactly what we need - will certainly need typing info) *)
 (*ONLY creates function symbols - so projections are just user-named functions essentially - spec should
   just be that this produces SOME function symbol of the right type*)
-Definition complete_projections (csl: list funsym) : list (funsym * list funsym) :=
-  let conv_c (c: funsym) :=
-    let conv_p (i: nat) (ty: vty) :=
-      let id := ((s_name c) ++ "_proj_" ++ (nat_to_string i))%string in
-      (*TODO: do we need option?*)(funsym_noconstr_noty id [f_ret c] ty)
-    in
-    (c, mapi conv_p (s_args c))
-  in
-  map conv_c csl.
 
+(*A functional version of the projection function symbol*)
+Definition projection_syms (c: funsym) : list funsym :=
+  let conv_p (i: nat) (ty: vty) :=
+    let id := ((s_name c) ++ "_proj_" ++ (nat_to_string i))%string in
+    (*TODO: do we need option?*)(funsym_noconstr_noty id [f_ret c] ty)
+  in
+  mapi conv_p (s_args c).
+
+
+Definition complete_projections (csl: list funsym) : list (funsym * list funsym) :=
+  map (fun c => (c, projection_syms c)) csl.
+
+(*Projection axioms*)
+(*We do NOT thread cp_map, pp_map*)
+
+(*What to do about [pp_map] - we do not have old projections.
+  Also we never access pp_map outside of this function - useless to us *)
+(*We consider projection axioms for a single constructor and list of projection symbols
+  (given by [projection_names]) - pj_add from before*)
+Definition projection_axioms (cc_map: amap funsym funsym) 
+  (cs: funsym) (pl: list funsym) : list (funsym * (string * formula)) :=
+  (* declare and define the projection functions *)
+  (*Fresh vars TODO*)
+  let vl := combine (gen_names (length (s_args cs)) "u" nil) (s_args cs) in
+  (* let vl = List.map (create_vsymbol (id_fresh "u")) cs.ls_args in *)
+  let tl := map Tvar vl in
+  let hd := tfun_infer' (amap_get_def funsym_eq_dec (cc_map) cs id_fs)
+    (map snd vl) tl in
+  (* let hd = fs_app (Mls.find cs state.cc_map) tl (Option.get cs.ls_value) in *)
+  (*TODO: added ty*)
+  (*NOTE: not creating new funsym because we don't have unique IDs, just use pj*)
+  let add (*(x: list funsym * amap funsym funsym * task)*) (tty: term * vty) (pj: funsym) :
+      (funsym * (string * formula)) :=
+      (* list funsym * amap funsym funsym * task := *)
+    let t := fst tty in let ty := snd tty in
+    (* let pj := option_get_Option.get pj in *)
+    (*NOTE: since we don't have unique ids, is this just pj? Is that a problem?*)
+    (* let ls := funsym_noconstr_noty (s_name pj) (s_args pj) (f_ret pj) in *)
+    let ls := pj in
+      (* match Mls.find pj pp_map with
+      | pj -> pj,pp_map
+      | exception Not_found ->
+        let id = id_clone pj.ls_name in
+        let ls = create_lsymbol id pj.ls_args pj.ls_value in
+        ls,Mls.add pj ls pp_map
+    in *)
+    (* let tsk := add_param_decl tsk ls in *) (*TODO*)
+    let id := ((s_name ls) ++ "'def")%string in
+    (* let id = id_derive (ls.ls_name.id_string ^ "'def") ls.ls_name in
+    let pr = create_prsymbol id in *)
+    let hh := tfun_infer' ls [(f_ret cs)] [hd] in
+    (* let hh = t_app ls [hd] t.t_ty in *)
+    let ax := fforalls vl (Feq ty hh t) in
+    (* let tsk := add_axiom tsk id ax in *) (*TODO*)
+    (*Ignore metas*)
+    (* let ax = t_forall_close vl [] (t_equ hh t) in
+    let tsk = add_prop_decl tsk Paxiom pr ax in
+    let tsk = add_meta_model_projection tsk ls in *)
+    (ls, (id, ax))
+  in
+  map2 add (combine tl (map snd vl)) pl.
+
+
+(*NOTE: this changed A LOT from the Why3 version, need to make sure it is correct (and possibly
+  harder to prove equivalent)*)
 Definition add_projections {A B: Type} (st: state * task) (_ts : A) (_ty : B) (csl: list funsym) :
   state * task :=
   let s := fst st in
   let tsk := snd st in
-  (* declare and define the projection functions *)
-  let pj_add x (y: funsym * _) :=
-    let '(cp_map,pp_map,tsk) := x in
-    let '(cs,pl) := y in
-    (*Fresh vars TODO*)
-    let vl := combine (gen_names (length (s_args cs)) "u" nil) (s_args cs) in
-    (* let vl = List.map (create_vsymbol (id_fresh "u")) cs.ls_args in *)
-    let tl := map Tvar vl in
-    let hd := tfun_infer' (amap_get_def funsym_eq_dec (s.(cc_map)) cs id_fs)
-      (map snd vl) tl in
-    (* let hd = fs_app (Mls.find cs state.cc_map) tl (Option.get cs.ls_value) in *)
-    (*TODO: added ty*)
-     let add (x: list funsym * amap funsym funsym * task) (tty: term * vty) (pj: funsym) :
-        list funsym * amap funsym funsym * task :=
-      let t := fst tty in let ty := snd tty in
-      let '(pjl,pp_map,tsk) := x in
-      (* let pj := option_get_Option.get pj in *)
-      let '(ls,pp_map) :=
-        match amap_get funsym_eq_dec pp_map pj with
-        | Some pj => (pj, pp_map)
-        | None =>
-          let id := (s_name pj) in
-          let ls := funsym_noconstr_noty id (s_args pj) (f_ret pj) in
-          (*NOTE: since we don't have unique ids, is this just pj? Is that a problem?*)
-          (ls, amap_set funsym_eq_dec pp_map pj ls)
-        end
-      in
-        (* match Mls.find pj pp_map with
-        | pj -> pj,pp_map
-        | exception Not_found ->
-          let id = id_clone pj.ls_name in
-          let ls = create_lsymbol id pj.ls_args pj.ls_value in
-          ls,Mls.add pj ls pp_map
-      in *)
-      let tsk := add_param_decl tsk ls in
-      let id := ((s_name ls) ++ "'def")%string in
-      (* let id = id_derive (ls.ls_name.id_string ^ "'def") ls.ls_name in
-      let pr = create_prsymbol id in *)
-      let hh := tfun_infer' ls [(f_ret cs)] [hd] in
-      (* let hh = t_app ls [hd] t.t_ty in *)
-      let ax := fforalls vl (Feq ty hh t) in
-      let tsk := add_axiom tsk id ax in
-      (*Ignore metas*)
-      (* let ax = t_forall_close vl [] (t_equ hh t) in
-      let tsk = add_prop_decl tsk Paxiom pr ax in
-      let tsk = add_meta_model_projection tsk ls in *)
-      (ls::pjl,pp_map,tsk)
-    in
-    let '(pjl,pp_map,tsk) := fold_left2' add (combine tl (map snd vl)) pl ([],pp_map,tsk)  in
-    (amap_set funsym_eq_dec cp_map cs (rev pjl), pp_map, tsk)
-  in
-  let csl := complete_projections csl in
-  let '(cp_map2, pp_map2, task) :=
-    fold_left pj_add csl (s.(cp_map), s.(pp_map), tsk)
-  in
-  (s <| cp_map := cp_map2 |> <|pp_map := pp_map2 |>, task).
+  (*For each constructor, get projections and axioms, add projection funsym and axioms to task*)
+  let tsk := fold_left (fun acc c => 
+    let projs := projection_axioms s.(cc_map) c (projection_syms c) in
+    fold_left (fun tsk x => 
+      let pj := fst x in
+      let ax := snd x in
+      add_axiom (add_param_decl tsk pj) (fst ax) (snd ax) 
+    ) projs acc
+    ) csl tsk in
+  (*update state with projections - should be just rev (projection_syms) (TODO make sure)*)
+  let cp_map2 := fold_left (fun acc x => amap_set funsym_eq_dec acc x (rev (projection_syms x))) csl s.(cp_map) in
+  let st := s <| cp_map := cp_map2 |> in
+  (st, tsk).
 
-Definition add_inversion (st: state * task) (ts: typesym) (ty: vty) (csl: list funsym) :
-  state * task :=
-  let s := fst st in let tsk := snd st in
-  if s.(no_inv) then st else
+(*TODO: do we need state at all (other than maybe constructor map) - we know exactly what is
+  in the state for each - really should just need task*)
+
+Definition inversion_axiom (cc_map: amap funsym funsym) 
+  (ts: typesym) (ty: vty) (csl: list funsym) : string * formula :=
   (* add the inversion axiom *)
   let ax_id := ((ts_name ts) ++ "_inversion")%string in
   (* let ax_pr = create_prsymbol (id_derive ax_id ts.ts_name) in *)
   (*TODO: fresh?*)
   let ax_vs := (gen_name "u"%string nil, ty) in 
   let ax_hd := Tvar ax_vs in
-  let mk_cs (cs: funsym) :=
-    let pjl := amap_get_def funsym_eq_dec s.(cp_map) cs nil in 
+  let mk_cs (cs: funsym) : formula :=
+    (*NOTE: we know the pjl from the projections*)
+    let pjl := rev (projection_syms cs) in
+    (* let pjl := amap_get_def funsym_eq_dec s.(cp_map) cs nil in  *)
     (*NOTE: change app to also give return type*)
     let app pj := tfun_infer_ret' pj [ty] [ax_hd] in
     (* let app pj = t_app_infer pj [ax_hd] in *)
-    let cs := amap_get_def funsym_eq_dec s.(cc_map) cs id_fs in
+    let cs := amap_get_def funsym_eq_dec cc_map cs id_fs in
     (* let cs = Mls.find cs state.cc_map in *)
     let pjl' := map app pjl in
     Feq ty ax_hd (tfun_infer' cs (map snd pjl') (map fst pjl'))
@@ -493,7 +550,15 @@ Definition add_inversion (st: state * task) (ts: typesym) (ty: vty) (csl: list f
   in
   let ax_f := map_join_left' Ftrue mk_cs (Fbinop Tor) csl in
   let ax_f := Fquant Tforall ax_vs ax_f (*t_forall_close [ax_vs] [] ax_f in*) in
-  (s, add_axiom tsk ax_id ax_f).
+  (ax_id, ax_f).
+
+
+Definition add_inversion (st: state * task) (ts: typesym) (ty: vty) (csl: list funsym) :
+  state * task :=
+  let s := fst st in let tsk := snd st in
+  if s.(no_inv) then st else
+  let inv := inversion_axiom s.(cc_map) ts ty csl in
+  (s, add_axiom tsk (fst inv) (snd inv)).
 
 (*TODO: since we don't have builtin projections, we can't do the
   [kept_no_case] part for projections. We don't implement it at all.
@@ -621,7 +686,7 @@ Variable (noind: bool) (noinv: bool) (nosel: bool).
 
 (*I suppose we could make all params, but prob not*)
 Definition empty_state : state := {| mt_map := amap_empty; cc_map := amap_empty;
-  cp_map := amap_empty; pp_map := amap_empty; no_ind := noind; no_inv := noinv; no_sel := nosel|}.
+  cp_map := amap_empty; (*pp_map := amap_empty;*) no_ind := noind; no_inv := noinv; no_sel := nosel|}.
 
 
 Definition eliminate_match : trans :=
